\documentclass[11pt]{article}
% 中文 \documentclass[UTF8]{ctexart}
% 编译快捷键：Command+Option+B

% 显示快捷键：Command+Option+V

% 正向搜索：选中代码Command+Option+J

% 反向搜索：shift+command点击预览PDF


\usepackage[utf8]{inputenc}


\usepackage{graphicx}


\usepackage{amsmath}
\usepackage{amssymb}
\usepackage{amsfonts}
\usepackage{amsthm}
\usepackage{mathrsfs}
\usepackage{bm}

\usepackage{physics}


\usepackage{enumerate}
\usepackage{hyperref}

\usepackage{verbatim}
\usepackage{url}
\usepackage{listings}
\usepackage{color} %red, green, blue, yellow, cyan, magenta, black, white





\usepackage[english]{babel}



\usepackage{mathtools}


\usepackage{geometry}

% \geometry{a4paper,scale=0.8}

\geometry{a4paper,left=2cm,right=2cm,top=2cm,bottom=3cm}

\usepackage{graphicx}
\usepackage{float}

\newcommand{\diag}{\mathop{\mathrm{diag}}}

\newcommand{\triu}{\mathop{\mathrm{triu}}}
\newcommand{\tril}{\mathop{\mathrm{tril}}}
\newcommand{\T}{\mathrm{T}}

\newcommand{\redtext}[1]{\textcolor{red}{#1}}

\newcommand{\bigzero}{\mbox{\normalfont\Large\bfseries 0}}
\newcommand{\rvline}{\hspace*{-\arraycolsep}\vline\hspace*{-\arraycolsep}}


\title{\textbf{MSc Project Notes}}
\author{\textit{Zhiwei Zhou}}
% \date{April 2022}

\begin{document}

\maketitle

\section{02.08.2022}
\subsection{Bidiagonal matrix}

\noindent Let $\tilde{U} \in \mathbb{R}^{n \times n}$ be a bidiagonal matrix with non-zero diagonal, 
$i.e. \ \tilde{u}_{ii} \neq 0 \ \text{for} \ i = 1, 2, \ldots , n$,

\begin{align*}
    \tilde{U} &= \mqty[
        \tilde{u}_{11} & \tilde{u}_{12} &   &   &  \\
          & \tilde{u}_{22} & \tilde{u}_{23} &   &  \\
          &   & \tilde{u}_{33} & \tilde{u}_{34} &  \\
          &   &   & \tilde{u}_{44} & \tilde{u}_{45}\\
          &   &   &   & \tilde{u}_{55}
        ]
\end{align*}

\noindent and $D = \diag(\tilde{u}_{ii})\ \text{for} \ i = 1, 2, \ldots , n$,


\begin{align*}
    D = \mqty[
        \frac{1}{\tilde{u}_{11}} &   &   &   &  \\
          & \frac{1}{\tilde{u}_{22}} &   &   &  \\
          &   & \frac{1}{\tilde{u}_{33}} &   &  \\
          &   &   & \frac{1}{\tilde{u}_{44}} &  \\
          &   &   &   & \frac{1}{\tilde{u}_{55}}
        ]
\end{align*}


\noindent replace $\frac{\tilde{u}_{i, i+1}}{\tilde{u}_{i+1, i+1}}$ by $u_{i, i+1}\ \text{for} \ i = 1, 2, \ldots , n-1$, and let $U = \tilde{U}D$,



\begin{align*}
    U &= \mqty[
        1 & \frac{\tilde{u}_{12}}{\tilde{u}_{22}} &   &   &  \\
          & 1 & \frac{\tilde{u}_{23}}{\tilde{u}_{33}} &   &  \\
          &   & 1 & \frac{\tilde{u}_{34}}{\tilde{u}_{44}} &  \\
          &   &   & 1 & \frac{\tilde{u}_{45}}{\tilde{u}_{55}}\\
          &   &   &   & 1
        ]\\
    &= \mqty[
        1 & u_{12} &   &   &  \\
          & 1 & u_{23} &   &  \\
          &   & 1 & u_{34} &  \\
          &   &   & 1 & u_{45}\\
          &   &   &   & 1
    ].
\end{align*}


\noindent Let $A = U^{-1}$ be the inverse of $U$, a upper triangular matrix,


\begin{align*}
    A = \mqty[
        a_{11} & a_{12} & a_{13} & a_{14} & a_{15}\\
          & a_{22} & a_{23} & a_{24} & a_{25}\\
          &   & a_{33} & a_{34} & a_{35}\\
          &   &   & a_{44} & a_{45}\\
          &   &   &   & a_{55}
        ]
\end{align*}
then $I = UU^{-1} = UA$,


\begin{align*}
    I = \mqty[
        1 &   &   &   &  \\
          & 1 &   &   &  \\
          &   & 1 &   &  \\
          &   &   & 1 &  \\
          &   &   &   & 1
        ]
    = \mqty[
        a_{11} & a_{12} + a_{22} u_{12} & a_{13} + a_{23} u_{12} & a_{14} + a_{24} u_{12} & a_{15} + a_{25} u_{12}\\
          & a_{22} & a_{23} + a_{33} u_{23} & a_{24} + a_{34} u_{23} & a_{25} + a_{35} u_{23}\\
          &   & a_{33} & a_{34} + a_{44} u_{34} & a_{35} + a_{45} u_{34}\\
          &   &   & a_{44} & a_{45} + a_{55} u_{45}\\
          &   &   &   & a_{55}
        ]
    = UA.
\end{align*}



\noindent Note that $UA = \diag(a_{ii}) + \triu(UA, 1)\ \text{for} \ i = 1, 2, \ldots , n$.

\noindent Find $A$ such that $\diag(a_{ii}) = I$ and $\triu(UA, 1) = 0_{n \times n}\ \text{for} \ i = 1, 2, \ldots , n$.

\begin{align*}
    xy^{\T} = \mqty[
        x_{1} y_{1} & x_{1} y_{2} & x_{1} y_{3} & x_{1} y_{4} & x_{1} y_{5}\\
        x_{2} y_{1} & x_{2} y_{2} & x_{2} y_{3} & x_{2} y_{4} & x_{2} y_{5}\\
        x_{3} y_{1} & x_{3} y_{2} & x_{3} y_{3} & x_{3} y_{4} & x_{3} y_{5}\\
        x_{4} y_{1} & x_{4} y_{2} & x_{4} y_{3} & x_{4} y_{4} & x_{4} y_{5}\\
        x_{5} y_{1} & x_{5} y_{2} & x_{5} y_{3} & x_{5} y_{4} & x_{5} y_{5}
    ]
\end{align*}


\noindent Express $A$ in form of an outer product, $i.e. \ A = xy^{\T}$ for $\forall x,y \in \mathbb{R}^{n}$, then
\begin{align*}
    \triu(UA, 1) = \triu(Uxy^{\T}, 1) = 0_{n \times n}
\end{align*}


% \begin{align*}
%     % A = xy^{\T} &= \mqty[
%     %     x_{1} y_{1} & x_{1} y_{2} & x_{1} y_{3} & x_{1} y_{4} & x_{1} y_{5}\\
%     %     x_{2} y_{1} & x_{2} y_{2} & x_{2} y_{3} & x_{2} y_{4} & x_{2} y_{5}\\
%     %     x_{3} y_{1} & x_{3} y_{2} & x_{3} y_{3} & x_{3} y_{4} & x_{3} y_{5}\\
%     %     x_{4} y_{1} & x_{4} y_{2} & x_{4} y_{3} & x_{4} y_{4} & x_{4} y_{5}\\
%     %     x_{5} y_{1} & x_{5} y_{2} & x_{5} y_{3} & x_{5} y_{4} & x_{5} y_{5}
%     % ]\\
%     A = \triu(xy^{\T}) &= \mqty[
%         x_{1} y_{1} & x_{1} y_{2} & x_{1} y_{3} & x_{1} y_{4} & x_{1} y_{5}\\
%           & x_{2} y_{2} & x_{2} y_{3} & x_{2} y_{4} & x_{2} y_{5}\\
%           &   & x_{3} y_{3} & x_{3} y_{4} & x_{3} y_{5}\\
%           &   &   & x_{4} y_{4} & x_{4} y_{5}\\
%           &   &   &   & x_{5} y_{5}
%     ]
% \end{align*}



% \noindent then, $UA = U\triu(xy^{\T}) = \diag(x_{i} y_{i}) + \triu(U\triu(xy^{\T}), 1)\ \text{for} \ i = 1, 2, \ldots , n$.


\noindent Note that $\triu(e_{n} y^{\T}, 1) = 0_{n \times n}$ as,

\begin{align*}
    e_{n} y^{\T} = \mqty[
         \\
         \\
         \\
         \\
        1
    ]
    \mqty[
        y_{1} & y_{2} & y_{3} & y_{4} & y_{5}
    ]
    = \mqty[
          &   &   &   &  \\
          &   &   &   &  \\
          &   &   &   &  \\
          &   &   &   &  \\
        y_{1} & y_{2} & y_{3} & y_{4} & y_{5}
    ]
\end{align*}

\noindent solve $Ux := e_{n}$ for $x$ by backward substitution, then let $y_{i} := \frac{1}{x_{i}}$ or $x_{i} y_{i} = 1\ \text{for} \ i = 1, 2, \ldots , n$.


\noindent Then,
\begin{align*}
    % UA &= U\triu(xy^{\T})\\
    % &= \diag(x_{i} y_{i}) + \triu(Uxy^{\T}, 1)\\
    UA &= \diag(a_{ii}) + \triu(UA, 1)\\
    &= \diag(x_{i} y_{i}) + \triu(Uxy^{\T}, 1)\\
    &= \diag(\underbrace{1, 1, \cdots, 1}_n) + \triu(e_{n} y^{\T}, 1)\\
    &= I + 0_{n \times n}\\
    &= I
\end{align*}



\subsection{Upper triangular matrix}

\noindent Let $\tilde{U} \in \mathbb{R}^{n \times n}$ be a banded matrix with non-zero diagonal, upper banded width $u$, and lower banded width $0$ 
\noindent Similarly,

\begin{align*}
    U = \mqty[
        1 & u_{12} & u_{13} &   &  \\
          & 1 & u_{23} & u_{24} &  \\
          &   & 1 & u_{34} & u_{35}\\
          &   &   & 1 & u_{45}\\
          &   &   &   & 1
    ]
\end{align*}

\begin{align*}
    UA &= \mqty[
        a_{11} & a_{12} + a_{22} u_{12} & a_{13} + a_{23} u_{12} + a_{33} u_{13} & a_{14} + a_{24} u_{12} + a_{34} u_{13} & a_{15} + a_{25} u_{12} + a_{35} u_{13}\\
          & a_{22} & a_{23} + a_{33} u_{23} & a_{24} + a_{34} u_{23} + a_{44} u_{24} & a_{25} + a_{35} u_{23} + a_{45} u_{24}\\
          &   & a_{33} & a_{34} + a_{44} u_{34} & a_{35} + a_{45} u_{34} + a_{55} u_{35}\\
          &   &   & a_{44} & a_{45} + a_{55} u_{45}\\
          &   &   &   & a_{55}
    ]\\
    &= \diag(a_{ii}) + \triu(UA, 1)\ \text{for} \ i = 1, 2, \ldots , n
\end{align*}

\noindent Find $A$ such that $\diag(a_{ii}) = I$ and $\triu(UA, 1) = 0_{n \times n}\ \text{for} \ i = 1, 2, \ldots , n$.

\begin{align*}
    XY^{\T} = \mqty[
        x_{11} y_{11} + x_{12} y_{12} & x_{11} y_{21} + x_{12} y_{22} & x_{11} y_{31} + x_{12} y_{32} & x_{11} y_{41} + x_{12} y_{42} & x_{11} y_{51} + x_{12} y_{52}\\
        x_{21} y_{11} + x_{22} y_{12} & x_{21} y_{21} + x_{22} y_{22} & x_{21} y_{31} + x_{22} y_{32} & x_{21} y_{41} + x_{22} y_{42} & x_{21} y_{51} + x_{22} y_{52}\\
        x_{31} y_{11} + x_{32} y_{12} & x_{31} y_{21} + x_{32} y_{22} & x_{31} y_{31} + x_{32} y_{32} & x_{31} y_{41} + x_{32} y_{42} & x_{31} y_{51} + x_{32} y_{52}\\
        x_{41} y_{11} + x_{42} y_{12} & x_{41} y_{21} + x_{42} y_{22} & x_{41} y_{31} + x_{42} y_{32} & x_{41} y_{41} + x_{42} y_{42} & x_{41} y_{51} + x_{42} y_{52}\\
        x_{51} y_{11} + x_{52} y_{12} & x_{51} y_{21} + x_{52} y_{22} & x_{51} y_{31} + x_{52} y_{32} & x_{51} y_{41} + x_{52} y_{42} & \redtext{x_{51}} y_{51} + x_{52} y_{52}
    ]
\end{align*}



\noindent Express $A$ in outer product, $i.e. \ A = XY^{\T}$, for $\forall X,Y \in \mathbb{R}^{n \times 2}$,


\begin{align*}
    \triu(UA, 1) = \triu(UXY^{\T}, 1) = 0_{n \times n}
\end{align*}


\noindent Note that $\triu(\mqty[e_{n-1} & e_{n}] Y^{\T}, \textcolor{red}{2}) = 0_{n \times n}$ as,

\begin{align*}
    \mqty[e_{n-1} & e_{n}] Y^{\T} = \mqty[
          &   \\
          &   \\
          &   \\
        1 &   \\
          & 1 \\
    ]
    \mqty[
        y_{11} & y_{21} & y_{31} & y_{41} & y_{51}\\
        y_{12} & y_{22} & y_{32} & y_{42} & y_{52}
    ]
    = \mqty[
          &   &   &   &  \\
          &   &   &   &  \\
          &   &   &   &  \\
        y_{11} & y_{21} & y_{31} & y_{41} & y_{51}\\
        y_{12} & y_{22} & y_{32} & y_{42} & y_{52}
    ]
\end{align*}


\noindent solve $UX = U\mqty[x_{1} & x_{2}] := \mqty[e_{n-1} & e_{n}]$ for $x_{1}$ and $x_{2}$ by backward substitution,
% \noindent then, $UA = U\triu(XY^{\T}) = U$?

\newpage
\section{09.06.2022}

\subsection{Notation}

\subsubsection*{Vectors}

\begin{align*}
    b = \mqty[
        b_{1} \\
        b_{2} \\
        \vdots \\
        b_{n}
        ]
    \in \mathbb{R}^n
\end{align*}


\subsubsection*{Matrices and Columns}

\begin{align*}
    A &= \mqty[
        a_{11} & a_{12} & \cdots & a_{1n} \\
        a_{21} & a_{22} & \cdots & a_{1n} \\
        \vdots & \vdots & \ddots & \vdots \\
        a_{m1} & a_{m2} & \cdots & a_{mn}
        ]\\
    &= \mqty[
        a_{1} & a_{2} & \cdots & a_{n}
        ]
    \in \mathbb{R}^{m \times n}
    ,\ a_{i} \in \mathbb{R}^{m}
\end{align*}

\begin{align*}
    Ae_{i} &:= a_{i}\\
    e_{i} &= i\text{-th column of }I\\
        % &= 
        % \begin{cases}
        %     dasdsa\\
        %     dsadsa
        % \end{cases}
\end{align*}

\subsubsection*{Block Matrices and Block Columns}

\begin{align*}
    A &= \mqty[
        A_{11} & A_{12} & \cdots & A_{1l} \\
        A_{21} & A_{22} & \cdots & A_{1l} \\
        \vdots & \vdots & \ddots & \vdots \\
        A_{k1} & A_{k2} & \cdots & A_{kl}
        ],\ A_{ij} \in \mathbb{R}^{m \times n} \\
    &= \mqty[
        A_{1} & A_{2} & \cdots & A_{l}
        ]
    \in \mathbb{R}^{km \times ln}
    ,\ A_{i} \in \mathbb{R}^{km \times n}
\end{align*}


\begin{align*}
    AE_{i} &\coloneqq A_{i}\\
    E_{i} &= i\text{-th block column of }I\\
        % &= 
        % \begin{cases}
        %     dasdsa\\
        %     dsadsa
        % \end{cases}
\end{align*}



\subsection{Bidiagonal matrix (upper)}




% \noindent Let $U \in \mathbb{R}^{n \times n}$ be a bidiagonal matrix with non-zero diagonal, 
% $i.e. \ u_{ii} \neq 0 \ \text{for} \ i = 1, 2, \ldots , n$,

\begin{align*}
    U &= \mqty[
        d_{1} & b_{1} &   &   &  \\
          & d_{2} & b_{2} &   &  \\
          &   & \ddots & \ddots &  \\
          &   &   & d_{n-1} & b_{n-1}\\
          &   &   &   & d_{n}
    ] \in \mathbb{R}^{n \times n}
\end{align*}




\begin{align*}
    x &= \mqty[
        x_{1} \\
        x_{2} \\
        \vdots \\
        x_{n-1} \\
        x_{n}
        ]
    \in \mathbb{R}^{n \times 1}
    &
    y &= \mqty[
        y_{1} \\
        y_{2} \\
        \vdots \\
        y_{n-1} \\
        y_{n}
        ]
    \in \mathbb{R}^{n \times 1}
    &
    y^{\T} &= \mqty[
        y_{1} & y_{2} & \cdots & y_{n-1} & y_{n}
        ] \in \mathbb{R}^{1 \times n}
\end{align*}



\begin{align*}
    xy^{\T} &= \mqty[
        x_{1} \\
        x_{2} \\
        \vdots \\
        x_{n-1} \\
        x_{n}
        ]
        \mqty[
        y_{1} & y_{2} & \cdots & y_{n-1} & y_{n}
        ]\\
    &= \mqty[
        x_{1} y_{1} & x_{1} y_{2} & \cdots & x_{1} y_{n-1} & x_{1} y_{n}\\
        x_{2} y_{1} & x_{2} y_{2} & \cdots & x_{2} y_{n-1} & x_{2} y_{n}\\
        \vdots & \vdots & \ddots & \vdots & \vdots\\
        x_{n-1} y_{1} & x_{n-1} y_{2} & \cdots & x_{n-1} y_{n-1} & x_{n-1} y_{n}\\
        x_{n} y_{1} & x_{n} y_{2} & \cdots & x_{n} y_{n-1} & x_{n} y_{n}
        ]\\
    &= x\mqty[
            y_{1} & y_{2} & \cdots & y_{n-1} & y_{n}
            ]\\
    &= \mqty[
        xy_{1} & xy_{2} & \cdots & xy_{n-1} & xy_{n}
        ]
\end{align*}




\begin{align*}
    \triu(xy^{\T}) &= \mqty[
        x_{1} y_{1} & x_{1} y_{2} & \cdots & x_{1} y_{n-1} & x_{1} y_{n}\\
        0 & x_{2} y_{2} & \cdots & x_{2} y_{n-1} & x_{2} y_{n}\\
        \vdots & \vdots & \ddots & \vdots & \vdots\\
        0 & 0 & \cdots & x_{4} y_{n-1} & x_{4} y_{n}\\
        0 & 0 & \cdots & 0 & x_{5} y_{n}
        ]\\
    &= \mqty[
        \mqty[
            x_{1:1} \\
            0_{n-1}
            ]y_{1} &
        \mqty[
            x_{1:2} \\
            0_{n-2}
            ]y_{2} &
        \cdots &
        \mqty[
            x_{1:n-1} \\
            0
            ]y_{n-1} &
        x y_{n} 
        ]
\end{align*}


\begin{align*}
    U^{-1} &= \triu(xy^{\T}) \\
    I &= U \triu(xy^{\T})
\end{align*}

$n$-th column, 
\begin{align*}
    e_{n} &= U \triu(xy^{\T})e_{n} \\
    &= U x y_{n}    
\end{align*}



% \begin{align*}
%     x :&= \alpha U^{-1} e_{n} \\
%     Ux &= \alpha e_{n} \\
%     e_{n} &= U x y_{n} \\
%         &= \alpha e_{n} y_{n} \\
%     y_n :&= \frac{1}{\alpha}
% \end{align*}

\begin{align*}
    x :&= U^{-1} e_{n} \\
    % e_{n} &= U x \\
    e_{n} &= U x y_{n} \\
        &= U U^{-1} e_{n} y_{n} \\
        &= e_{n} y_{n} \\
    y_n :&= 1
\end{align*}


$(n-1)$-th column, 

\begin{align*}
    e_{n-1} &= U \triu(xy^{\T})e_{n-1} \\
    &= U \mqty[
        x_{1:n-1} \\
        0
        ]y_{n-1}   
\end{align*}

$(n-1)$-th row of $(n-1)$-th column, 

\begin{align*}
    e_{i}^{\T} e_{j} = \delta_{ij} 
\end{align*}

\begin{align*}
    e_{n-1}^{\T} e_{n-1} = 1 &= e_{n-1}^{\T} U \mqty[
        x_{1:n-1} \\
        0
        ]y_{n-1} \\
        &= \mqty[
            0_{n-2} & d_{n-1} & b_{n-1}
        ] \mqty[
            x_{1:n-1} \\
            0
        ]y_{n-1} \\
        & = d_{n-1} x_{n-1} y_{n-1} \\
    y_{n-1} :&= (d_{n-1} x_{n-1})^{-1}
\end{align*}


\begin{align*}
    % x :&= U^{-1} e_n\\
    e_{n} &= U x \\
    e_{n}^{\T} e_{n} = 1 &= e_{n}^{\T} U x \\
        &= \mqty[
            0_{n-1} & d_{n}
        ] x \\
        &= d_{n} x_{n} \\
    y_{n} :&= 1 \\
        :&= (d_{n} x_{n})^{-1}
    % y_{n-1} :&= (d_{n-1} x_{n-1})^{-1}
\end{align*}

\begin{align*}
    x :&= U^{-1} e_n \\
    y_{i} :&= (d_{i} x_{i})^{-1}
\end{align*}



% \noindent Let $x \in \mathbb{R}^{n}$

\newpage
\subsection{Tridiagonal matrix (Upper)}




% \noindent Let $U \in \mathbb{R}^{n \times n}$ be a bidiagonal matrix with non-zero diagonal, 
% $i.e. \ u_{ii} \neq 0 \ \text{for} \ i = 1, 2, \ldots , n$,


$n = 2k$

\begin{align*}
    U &= \mqty[
        d_{1} & b^{1}_{1} & b^{2}_{1} &   &   &   &   &   &  \\
          & d_{2} & b^{1}_{2} & b^{2}_{2} &   &   &   &   &  \\
          &   & d_{3} & b^{1}_{3} & b^{2}_{3} &   &   &   &  \\
          &   &   & d_{4} & b^{1}_{4} & b^{2}_{4} &   &   &  \\
          &   &   &   & \ddots & \ddots & \ddots &   &  \\
          &   &   &   &   & d_{n-3} & b^{1}_{n-3} & b^{2}_{n-3} &  \\
          &   &   &   &   &   & d_{n-2} & b^{1}_{n-2} & b^{2}_{n-2}\\
          &   &   &   &   &   &   & d_{n-1} & b^{1}_{n-1}\\
          &   &   &   &   &   &   &   & d_{n}
    ]\\
    &= \mqty[
        \mqty[d_{1} & b^{1}_{1} \\ & d_{2}] & \mqty[b^{2}_{1} &  \\ b^{1}_{2} & b^{2}_{2}] &   &   &  \\
          & \mqty[d_{3} & b^{1}_{3} \\ & d_{4}] & \mqty[b^{2}_{3} & \\ b^{1}_{4} & b^{2}_{4}] &   &  \\
          &   & \ddots & \ddots &  \\
          &   &   & \mqty[d_{2k-3} & b^{1}_{2k-3} \\ & d_{2k-2}] & \mqty[b^{2}_{2k-3} & \\ b^{1}_{2k-2} & b^{2}_{2k-2}] \\
          &   &   &   & \mqty[d_{2k-1} & b^{1}_{2k-1}\\ & d_{2k}]
    ]\\
    &= \mqty[
        D_{1} & B_{1} &   &   &  \\
          & D_{2} & B_{2} &   &  \\
          &   & \ddots & \ddots &  \\
          &   &   & D_{k-1} & B_{k-1}\\
          &   &   &   & D_{k}
    ] \in \mathbb{R}^{2k \times 2k}
\end{align*}

\begin{align*}
    X &= \mqty[
        X_{1} \\
        X_{2} \\
        \vdots \\
        X_{k-1} \\
        X_{k}
        ]
    \in \mathbb{R}^{2k \times 2}
    &
    Y &= \mqty[
        Y_{1} \\
        Y_{2} \\
        \vdots \\
        Y_{k-1} \\
        Y_{k}
        ]
    \in \mathbb{R}^{2k \times 2}
    &
    Y^{\T} &= \mqty[
        Y_{1}^{\T} & Y_{2}^{\T} & \cdots & Y_{k-1}^{\T} & Y_{k}^{\T}
        ] \in \mathbb{R}^{2 \times 2k}
\end{align*}



\begin{align*}
    XY^{\T} &= \mqty[
        X_{1} \\
        X_{2} \\
        \vdots \\
        X_{k-1} \\
        X_{k}
        ]
        \mqty[
        Y_{1}^{\T} & Y_{2}^{\T} & \cdots & Y_{k-1}^{\T} & Y_{k}^{\T}
        ]\\
    &= \mqty[
        X_{1} Y_{1}^{\T} & X_{1} Y_{2}^{\T} & \cdots & X_{1} Y_{k-1}^{\T} & x_{1} Y_{k}^{\T}\\
        X_{2} Y_{1}^{\T} & X_{2} Y_{2}^{\T} & \cdots & X_{2} Y_{k-1}^{\T} & x_{2} Y_{k}^{\T}\\
        \vdots & \vdots & \ddots & \vdots & \vdots\\
        X_{k-1} Y_{1}^{\T} & X_{k-1} Y_{2}^{\T} & \cdots & X_{k-1} Y_{k-1}^{\T} & X_{k-1} Y_{k}^{\T}\\
        X_{k} Y_{1}^{\T} & X_{k} Y_{2}^{\T} & \cdots & X_{k} Y_{k-1}^{\T} & X_{k} Y_{k}^{\T}
        ]\\
    &= X\mqty[
        Y_{1}^{\T} & Y_{2}^{\T} & \cdots & Y_{k-1}^{\T} & Y_{k}^{\T}
            ]\\
    &= \mqty[
        XY_{1}^{\T} & XY_{2}^{\T} & \cdots & XY_{k-1}^{\T} & XY_{k}^{\T}
        ]
\end{align*}

\begin{align*}
    \triu(X_{k}) &\coloneqq X_{k} \\
    \triu(Y_{k}^{\T}) &\coloneqq Y_{k}^{\T} \\
    \triu(X_{k} Y_{k}^{\T}) &= X_{k} Y_{k}^{\T}
\end{align*}

\begin{align*}
    \triu(XY^{\T}) &= \mqty[
        \triu(X_{1} Y_{1}^{\T}) & X_{1} Y_{2}^{\T} & \cdots & X_{1} Y_{k-1}^{\T} & X_{1} Y_{k}^{\T}\\
        0_{2 \times 2} & \triu(X_{2} Y_{2}^{\T}) & \cdots & X_{2} Y_{k-1}^{\T} & X_{2} Y_{k}^{\T}\\
        \vdots & \vdots & \ddots & \vdots & \vdots\\
        0_{2 \times 2} & 0_{2 \times 2} & \cdots & \triu(X_{k-1} Y_{k-1}^{\T}) & X_{k-1} Y_{k}^{\T}\\
        0_{2 \times 2} & 0_{2 \times 2} & \cdots & 0_{2 \times 2} & X_{k} Y_{k}^{\T}
        ]\\
    &= \mqty[
        \mqty[
            \triu(X_{1} Y_{1}^{\T}) \\
            0_{2(k-1) \times 2}
            ] &
        \mqty[
            X_{1} Y_{2}^{\T} \\
            \triu(X_{2} Y_{2}^{\T}) \\
            0_{2(k-2) \times 2}
            ] &
        \cdots &
        \mqty[
            X_{1:k-2}Y_{k-1}^{\T} \\
            \triu(X_{k-1}Y_{k-1}^{\T}) \\
            0_{2 \times 2}
            ] &
        X Y_{k}^{\T}
        ]
\end{align*}


\begin{align*}
    U^{-1} &= \triu(XY^{\T}) \\
    I &= U \triu(XY^{\T})
\end{align*}

\begin{align*}
    E_{i} &= \mqty[0 & \cdots & 0 & I_{2 \times 2} & 0 & \cdots & 0]^{\T}
\end{align*}




$k$-th block column, 
\begin{align*}
    E_{k} &= U \triu(XY^{\T})E_{k} \\
    &= U X Y_{k}^{\T}
\end{align*}


\begin{align*}
    X &\coloneqq U^{-1} E_{k} \\
    % e_{n} &= U x \\
    E_{k} &= U X Y_{k}^{\T} \\
        &= U U^{-1} E_{k} Y_{k}^{\T} \\
        &= E_{k} Y_{k}^{\T} \\
    Y_{k}^{\T} &\coloneqq I_{2 \times 2}
\end{align*}


$(k-1)$-th block column, 

\begin{align*}
    E_{k-1} &= U \triu(XY^{\T})E_{k-1} \\
    &= U \mqty[
        X_{1:k-2}Y_{k-1}^{\T} \\
        \triu(X_{k-1}Y_{k-1}^{\T}) \\
        0_{2 \times 2}
        ]
\end{align*}

$(k-1)$-th block row of $(k-1)$-th block column, 

\begin{align*}
    E_{i}^{\T} E_{j} = 
    \begin{cases}
        I_{2 \times 2}, & \text{if} \ i=j \ ;\\
        0_{2 \times 2}, & \text{otherwise}.
    \end{cases} 
\end{align*}

\begin{align*}
    E_{k-1}^{\T} E_{k-1} = I_{2 \times 2} &= E_{k-1}^{\T} U \mqty[
        X_{1:k-2}Y_{k-1}^{\T} \\
        \triu(X_{k-1}Y_{k-1}^{\T}) \\
        0_{2 \times 2}
        ] \\
        &= \mqty[
            0_{2 \times 2(k-2)} & D_{k-1} & B_{k-1}
        ] \mqty[
            X_{1:k-2}Y_{k-1}^{\T} \\
            \triu(X_{k-1}Y_{k-1}^{\T}) \\
            0_{2 \times 2}
            ] \\
        & = D_{k-1} \triu(X_{k-1}Y_{k-1}^{\T}) \\
        % &= \triu(D_{k-1}X_{k-1}Y_{k-1}^{\T}) \ (\text{as}\  D_{k-1} = \triu(D_{k-1}))\\
    Y_{k-1}^{\T} &\coloneqq (D_{k-1} X_{k-1})^{-1}
\end{align*}

\begin{align*}
    D_{k-1} &= \triu(D_{k-1})\\
    D_{k-1}^{-1} &= \triu(D_{k-1}^{-1})\\
    Y_{k-1}^{\T} &\coloneqq (D_{k-1} X_{k-1})^{-1}\\
    D_{k-1} \triu(X_{k-1}Y_{k-1}^{\T}) &= D_{k-1} \triu(X_{k-1}(D_{k-1} X_{k-1})^{-1})\\
        &= D_{k-1} \triu(X_{k-1} X_{k-1}^{-1} D_{k-1}^{-1})\\
        &= D_{k-1} \triu(D_{k-1}^{-1})\\
        &= D_{k-1} D_{k-1}^{-1}\\
        &= I_{2 \times 2}
\end{align*}


\begin{align*}
    X &\coloneqq U^{-1} E_k\\
    E_{k} &= U X \\
    E_{k}^{\T} E_{k} = I_{2 \times 2} &= E_{k}^{\T} U X \\
        &= \mqty[
            0_{2 \times 2(k-1)} & D_{k}
        ] X \\
        &= D_{k} X_{k} \\
    Y_{k} &\coloneqq I_{2 \times 2} \\
        &\coloneqq (D_{k} X_{k})^{-1}
    % y_{n-1} :&= (d_{n-1} x_{n-1})^{-1}
\end{align*}

\begin{align*}
    X &\coloneqq U^{-1} E_{k} \\
    Y_{i} &\coloneqq (D_{i} X_{i})^{-1}
\end{align*}









\newpage
$n = 2k + 1$
\begin{align*}
    U &= \mqty[
        \mqty[d_{1}] & \mqty[b^{1}_{1} & b^{2}_{1}] &   &   &  \\
          & \mqty[d_{2} & b^{1}_{2} \\ & d_{3}] & \mqty[b^{2}_{2} & \\ b^{1}_{3} & b^{2}_{3}] &   &  \\
          &   & \ddots & \ddots &  \\
          &   &   & \mqty[d_{2k-2} & b^{1}_{2k-2} \\ & d_{2k-1}] & \mqty[b^{2}_{2k-2} & \\ b^{1}_{2k-1} & b^{2}_{2k-1}] \\
          &   &   &   & \mqty[d_{2k} & b^{1}_{2k}\\ & d_{2k+1}]
    ]\\
    &= \mqty[
        \tilde{D_{0}} & \tilde{B_{0}} &   &   &  \\
          & D_{1} & B_{1} &   &  \\
          &   & \ddots & \ddots &  \\
          &   &   & D_{k-1} & B_{k-1}\\
          &   &   &   & D_{k}
    ] \in \mathbb{R}^{(2k+1) \times (2k+1)}
\end{align*}




% \begin{equation}
%     \left[\begin{array}{ll|ll|l}
%     a & b & c & & \\
%     & d & e & f & \\
%     \hline & & g & h & i \\
%     & & j & R \\
%     \hline & & l
%     \end{array}\right]
% \end{equation}








\end{document}




